Modal/modal/logics/logic_E.lean
@@ -1,4 +1,4 @@
-import Modal.cpl.cpl
+import Modal.cpl.entailment
 import Modal.modal.common.formula
 import Modal.modal.common.axioms_rules
 
@@ -12,12 +12,8 @@ inductive EProof : Set (Formula 𝓐) → Formula 𝓐 → Prop where
       (h : p ∈ Γ) :
       EProof Γ p
   | cpl {Γ : Set (Formula 𝓐)} {φ : Formula 𝓐}
-      (h_cpl : (CPL.Entailment (Formula 𝓐)).entails ∅ ((to_cpl 𝓐) φ)) :
+      (h_cpl : (CPL.entails ∅ ((to_cpl 𝓐) φ))) :
       EProof Γ φ
   | re {Γ : Set (Formula 𝓐)} {φ ψ : Formula 𝓐}
       (h_prem : EProof Γ (Rules.re φ ψ).premise) :
       EProof Γ (Rules.re φ ψ).conclusion
-
-def EEntailment : EntailmentSystem :=
-  { formula := Formula 𝓐
-    entails := EProof }
