Modal/modal/models/kripke.lean
@@ -1,5 +1,4 @@
-import Modal.cpl.proof
-import Modal.modal.formula
+import Modal.modal.common.formula
 
 
 namespace Kripke
@@ -11,36 +10,35 @@ structure Frame where
   world : Type
   rel : world → world → Prop
 
--- α is the set of atomic propositions
-structure Model (α : Type) where
+-- 𝓐 is the set of atomic propositions
+structure Model (𝓐 : Type) where
   frame : Frame
-  val : frame.world → α → Prop
+  val : frame.world → 𝓐 → Prop
 
 
-
-variable {α : Type}
+variable {𝓐 : Type}
 
 -- Defines truth at a specific world w, that is m, w ⊨ φ.
-def world_sat (m : Model α) (w : m.frame.world) : Modal.Formula α → Prop
+def world_sat (m : Model 𝓐) (w : m.frame.world) : Modal.Formula 𝓐 → Prop
   | .atom a   => m.val w a
   | .bot      => False
   | .impl φ ψ => world_sat m w φ → world_sat m w ψ
   | .box φ    => ∀ v, m.frame.rel w v → world_sat m v φ
 
 -- Defines truth in an entire model m, that is m ⊨ φ.
-def model_sat (m : Model α) (φ : Modal.Formula α) : Prop :=
+def model_sat (m : Model 𝓐) (φ : Modal.Formula 𝓐) : Prop :=
   ∀ w, world_sat m w φ
 
 -- Defines truth in an entire model f, that is f ⊨ φ.
-def frame_sat (f : Frame) (φ : Modal.Formula α) : Prop :=
+def frame_sat (f : Frame) (φ : Modal.Formula 𝓐) : Prop :=
   ∀ val, model_sat ⟨f, val⟩ φ
 
 -- Defines truth in all possible models, that is ⊨ φ.
-def valid (φ : Modal.Formula α) : Prop :=
+def valid (φ : Modal.Formula 𝓐) : Prop :=
   ∀ (f : Frame), frame_sat f φ
 
 -- Defines truth in all frames satisfying a given class/property.
-def valid_in_class (P : Frame → Prop) (φ : Modal.Formula α) : Prop :=
+def valid_in_class (P : Frame → Prop) (φ : Modal.Formula 𝓐) : Prop :=
   ∀ (f : Frame), P f → frame_sat f φ
 
 end Kripke
