Modal.lean
@@ -1,19 +1,23 @@
--- import Modal.Basic  -- it is empty at the moment
+-- import Modal.Basic  -- empty at the moment
 
 -- common utilities
-import Modal.common.inference
-import Modal.common.entailment
 import Modal.common.consistency
+import Modal.common.entailment
+import Modal.common.inference
+import Modal.common.modeling
+import Modal.common.syntax
 
--- classical propositional logic (CPL)
-import Modal.cpl.syntax
+-- classical propositional logic
+import Modal.cpl.entailment
 import Modal.cpl.formula
-import Modal.cpl.cpl
+import Modal.cpl.modeling
+import Modal.cpl.sound_complete
+import Modal.cpl.syntax
 
 -- modal logic
-import Modal.modal.common.syntax
-import Modal.modal.common.formula
 import Modal.modal.common.axioms_rules
+import Modal.modal.common.formula
+import Modal.modal.common.syntax
 
 -- modal logic systems
 import Modal.modal.logics.logic_E
@@ -21,12 +25,12 @@ import Modal.modal.logics.logic_K
 import Modal.modal.logics.logic_M
 
 -- models
---import Modal.modal.models.kripke
---import Modal.modal.models.nbhd
---import Modal.modal.models.dual
+import Modal.modal.models.dual
+import Modal.modal.models.kripke_new
+import Modal.modal.models.nbhd_new
 
 -- soundness and completeness results
---import Modal.modal.sound_complete.logicK_kripke
+import Modal.modal.sound_complete.logicE_nbhd
+import Modal.modal.sound_complete.logicK_kripke
 --import Modal.modal.sound_complete.logicM_dual
---import Modal.modal.sound_complete.logicM_upnbhd
---import Modal.modal.sound_complete.logicE_nbhd
+import Modal.modal.sound_complete.logicM_upnbhd
