Modal/common/modeling.lean
@@ -1,0 +1,6 @@
+import Mathlib.Data.Set.Basic
+
+
+class HasModels (𝓕 : Type) where
+  models : Set 𝓕 → 𝓕 → Prop
+notation Γ " ⊨ " φ:50 => HasModels.models Γ φ
