Modal/common/syntax.lean
@@ -1,0 +1,8 @@
+namespace Common.Syntax
+
+class HasBot (𝓕 : Type) where
+  bot : 𝓕
+
+notation "⊥" => HasBot.bot
+
+end Common.Syntax
