Modal/cpl/entailment.lean
@@ -1,0 +1,17 @@
+/- At the moment, I do not care how entailment is defined
+for CPL. I only assume there is some definition for it
+that satisfies the needed metatheorems. -/
+
+import Modal.cpl.formula
+import Modal.common.entailment
+import Modal.common.modeling
+
+namespace CPL
+open Formula
+
+variable {𝓐 : Type}
+
+def entails : Set (Formula 𝓐) → Formula 𝓐 → Prop := by admit
+instance : HasEntails (Formula 𝓐) where entails := entails
+
+end CPL
