Modal/cpl/sound_complete.lean
@@ -1,0 +1,16 @@
+import Modal.cpl.entailment
+import Modal.cpl.modeling
+
+
+namespace CPL
+
+theorem sound {𝓐 : Type} {Γ : Set (Formula 𝓐)} {φ : Formula 𝓐}
+        (h : CPL.entails Γ φ) : (CPL.models Γ φ) :=
+    by admit
+
+
+theorem complete {𝓐 : Type} {Γ : Set (Formula 𝓐)} {φ : Formula 𝓐}
+        (h : CPL.models Γ φ) : (CPL.entails Γ φ) :=
+    by admit
+
+end CPL
