Modal/cpl/syntax.lean
@@ -1,6 +1,7 @@
 /- I use 𝓕 (backslash MCF) for the type of formulas...
 or whatever is amenable to be used in its stead. -/
 
+import Modal.common.syntax
 
 namespace CPL
 
@@ -17,7 +18,6 @@ def and {𝓕 : Type} [Syntax 𝓕] (p q : 𝓕) : 𝓕 := neg (impl p (neg q))
 def iff {𝓕 : Type} [Syntax 𝓕] (p q : 𝓕) : 𝓕 := and (impl p q) (impl q p)
 
 
-notation  "⊥"   => bot
 notation  "⊤"   => top
 prefix:40 "¬"   => neg
 infixr:35 " ∧ " => and
@@ -26,6 +26,14 @@ infixr:20 " → " => impl
 infixl:20 " ↔ " => iff
 -- precedence levels: higher binds tighter
 -- 40 (¬), 35 (∧), 30 (∨), 20 (→, ↔)
+
+instance {𝓕 : Type} [Syntax 𝓕] : Common.Syntax.HasBot 𝓕 where bot := Syntax.bot
+
+class HasImpl (𝓕 : Type) where
+  impl : 𝓕 → 𝓕 → 𝓕
+
+class HasBox (𝓕 : Type) where
+  box : 𝓕 → 𝓕
 
 end Syntax
 
