Modal/modal/models/kripke_new.lean
@@ -1,0 +1,51 @@
+import Modal.modal.common.formula
+import Modal.cpl.syntax
+import Modal.common.syntax
+
+
+namespace Kripke
+
+open CPL.Syntax Common.Syntax
+
+structure Frame where
+  world : Type
+  rel : world → world → Prop
+
+-- We assume a `sat` function that tells whether a formula is satisfied at a world.
+-- We also assume that this `sat` function respects the connectives.
+-- This is in contrast to the more usual approach of defining `sat` inductively,
+-- starting from a valuacion of atomic propositions.
+structure Model (𝓕 : Type) [HasBot 𝓕] [HasImpl 𝓕] [HasBox 𝓕] where
+  frame : Frame
+  sat : frame.world → 𝓕 → Prop
+  h_bot : ∀ w, ¬(sat w HasBot.bot)
+  h_impl : ∀ w φ ψ, (sat w (HasImpl.impl φ ψ)) ↔ (sat w φ → sat w ψ)
+  h_box : ∀ w φ, (sat w (HasBox.box φ)) ↔ (∀ v, frame.rel w v → sat v φ)
+
+variable {𝓕 : Type} [HasBot 𝓕] [HasImpl 𝓕] [HasBox 𝓕]
+
+-- Defines truth at a specific world w, that is m, w ⊨ φ.
+def world_sat (m : Model 𝓕) (w : m.frame.world) : 𝓕 → Prop :=
+  fun φ => m.sat w φ
+
+-- Defines truth in an entire model m, that is m ⊨ φ.
+def model_sat (m : Model 𝓕) (φ : 𝓕) : Prop :=
+  ∀ w, world_sat m w φ
+
+-- Defines truth in an entire model f, that is f ⊨ φ.
+def frame_sat (f : Frame) (φ : 𝓕) : Prop :=
+  ∀ (sat : f.world → 𝓕 → Prop)
+    (h_bot : ∀ w, ¬(sat w HasBot.bot))
+    (h_impl : ∀ w φ ψ, (sat w (HasImpl.impl φ ψ)) ↔ (sat w φ → sat w ψ))
+    (h_box : ∀ w φ, (sat w (HasBox.box φ)) ↔ (∀ v, f.rel w v → sat v φ)),
+    model_sat ⟨f, sat, h_bot, h_impl, h_box⟩ φ
+
+-- Defines truth in all possible models, that is ⊨ φ.
+def valid (φ : 𝓕) : Prop :=
+  ∀ (f : Frame), frame_sat f φ
+
+-- Defines truth in all frames satisfying a given class/property.
+def valid_in_class (P : Frame → Prop) (φ : 𝓕) : Prop :=
+  ∀ (f : Frame), P f → frame_sat f φ
+
+end Kripke
