Modal/modal/models/nbhd_new.lean
@@ -1,0 +1,52 @@
+import Modal.modal.common.formula
+import Modal.cpl.syntax
+import Modal.common.syntax
+
+
+namespace Neighborhood
+
+open CPL.Syntax Common.Syntax
+
+
+structure Frame where
+  world : Type
+  nbhd : world → Set (Set world)
+
+structure Model (𝓕 : Type) [HasBot 𝓕] [HasImpl 𝓕] [HasBox 𝓕] where
+  frame : Frame
+  sat : frame.world → 𝓕 → Prop
+  h_bot : ∀ w, ¬(sat w HasBot.bot)
+  h_impl : ∀ w φ ψ, (sat w (HasImpl.impl φ ψ)) ↔ (sat w φ → sat w ψ)
+  h_box : ∀ w φ, {v | sat v φ} ∈ frame.nbhd w
+
+class IsUpwardClosed (f : Frame) : Prop where
+  is_up_closed : ∀ w (X Y : Set f.world), X ∈ f.nbhd w → X ⊆ Y → Y ∈ f.nbhd w
+
+
+variable {𝓕 : Type} [HasBot 𝓕] [HasImpl 𝓕] [HasBox 𝓕]
+
+-- Defines truth at a specific world w, that is m, w ⊨ φ.
+def world_sat (m : Model 𝓕) (w : m.frame.world) : 𝓕 → Prop :=
+  fun φ => m.sat w φ
+
+-- Defines truth in an entire model m, that is m ⊨ φ.
+def model_sat (m : Model 𝓕) (φ : 𝓕) : Prop :=
+  ∀ w, world_sat m w φ
+
+-- Defines truth in an entire frame f, that is f ⊨ φ.
+def frame_sat (f : Frame) (φ : 𝓕) : Prop :=
+  ∀ (sat : f.world → 𝓕 → Prop)
+    (h_bot : ∀ w, ¬(sat w HasBot.bot))
+    (h_impl : ∀ w φ ψ, (sat w (HasImpl.impl φ ψ)) ↔ (sat w φ → sat w ψ))
+    (h_box : ∀ w φ, {v | sat v φ} ∈ f.nbhd w),
+    model_sat ⟨f, sat, h_bot, h_impl, h_box⟩ φ
+
+-- Defines truth in all possible models, that is ⊨ φ.
+def valid (φ : 𝓕) : Prop :=
+  ∀ (f : Frame), frame_sat f φ
+
+-- Defines truth in all frames satisfying a given class/property.
+def valid_in_class (P : Frame → Prop) (φ : 𝓕) : Prop :=
+  ∀ (f : Frame), P f → frame_sat f φ
+
+end Neighborhood
