Modal/modal/sound_complete/logicE_nbhd.lean
@@ -1,12 +1,12 @@
-import Modal.modal.formula
-import Modal.modal.models.nbhd
+import Modal.modal.common.formula
+import Modal.modal.models.nbhd_new
 import Modal.modal.logics.logic_E
 
 
-variable {α : Type}
+variable {𝓐 : Type}
 
 -- Soundness and completeness of logic E with respect to neighborhood models
 -- Well-known result
 theorem logicE_nbhd_sc :
-    ∀ (φ : Modal.Formula α), Neighborhood.valid φ ↔ EProof φ := by
-    admit
+    ∀ (φ : Modal.Formula 𝓐), Neighborhood.valid φ ↔ EProof (∅ : Set (Modal.Formula 𝓐)) φ := by
+  admit
