Modal/modal/sound_complete/logicK_kripke.lean
@@ -1,12 +1,12 @@
-import Modal.modal.formula
-import Modal.modal.models.kripke
+import Modal.modal.common.formula
+import Modal.modal.models.kripke_new
 import Modal.modal.logics.logic_K
 
 
-variable {α : Type}
+variable {𝓐 : Type}
 
 -- Soundness and completeness of logic K with respect to Kripke models
--- Well-known result
+-- Well-known result.
 theorem logicK_kripke_sc :
-    ∀ (φ : Modal.Formula α), Kripke.valid φ ↔ KProof φ := by
-    admit
+    ∀ (φ : Modal.Formula 𝓐), Kripke.valid φ ↔ KProof (∅ : Set (Modal.Formula 𝓐)) φ := by
+  admit
